done but for one admit

dev2015/dot21.v
@@ -1,8 +1,8 @@
 (* Full safety for DOT *)
 
-(* this version is based on dot19.v *)
-(* based on that, it makes methods have type TAll and removes ttapp and ttabs,  *)
-(* a first step towards fully dependent method types *)
+(* this version is based on dot20.v *)
+(* based on that, it adds the t_app_var typing rule, for  *)
+(* fully dependent method types *)
 
 Require Export SfLib.
 
@@ -348,6 +348,12 @@ Inductive has_type : tenv -> tm -> ty -> Prop :=
            has_type env x T1 ->
            stp env [] T2 T2 ->
            has_type env (tapp f l x) T2
+| t_app_var: forall env f l x T1 T2 T2X,
+           has_type env f (TAll l T1 T2) ->
+           has_type env (tvar x) T1 ->
+           open (varF x) T2 = T2X ->
+           stp env [] T2X T2X ->
+           has_type env (tapp f l (tvar x)) T2X
 | t_let: forall env x ex e Tx T,
            has_type env ex Tx ->
            fresh env <= x ->
@@ -7359,6 +7365,108 @@ Grab Existential Variables.
 apply 0. apply 0.
 Qed.
 
+Lemma invert_obj_var: forall venv vf l T1 T2 n vx nx xarg,
+  val_type venv vf (TAll l T1 T2) n ->
+  val_type venv vx T1 nx ->
+  index xarg venv = Some vx ->
+  sstpd2 true venv (open (varF xarg) T2) venv (open (varF xarg) T2) [] ->
+  exists env tenv TF ds x y T3 T4,
+    vf = (vobj env (fresh env) ds) /\
+    1 + (fresh env) = x /\
+    index l ds = Some (dfun x y) /\
+    wf_env env tenv /\
+    dcs_has_type (((fresh env), (open (varF (fresh env)) TF))::tenv) (fresh env) ds TF /\
+    sstpd2 true ((fresh env, vobj env (fresh env) ds) :: env) (open (varF (fresh env)) TF) ((fresh env, vobj env (fresh env) ds) :: env) (open (varF (fresh env)) TF) [] /\
+    has_type ((x,(open (varF (fresh env)) T3))::((fresh env),(open (varF (fresh env)) TF))::tenv) y (open (varF x) (open_rec 1 (varF (fresh env)) T4)) /\
+    sstpd2 true venv T1 (((fresh env), vobj env (fresh env) ds)::env) (open (varF (fresh env)) T3) [] /\
+    sstpd2 true ((x, vx)::((fresh env), vobj env (fresh env) ds)::env) (open (varF x) (open_rec 1 (varF (fresh env)) T4)) venv (open (varF xarg) T2) [].
+Proof.
+  intros. inversion H; repeat ev; try solve by inversion.
+  subst.
+  exists venv1. exists tenv0. exists T. exists ds.
+  assert (exists y T3 T4, index l ds = Some (dfun (1 + (fresh venv1))  y) /\ has_type ((1+(fresh venv1), (open (varF (fresh venv1)) T3)) :: ((fresh venv1), (open (varF (fresh venv1)) T)) :: tenv0) y (open (varF (1 + (fresh venv1))) (open_rec 1 (varF (fresh venv1)) T4)) /\ sstpd2 true (((fresh venv1), vobj venv1 (fresh venv1) ds)::venv1) (open (varF (fresh venv1)) (TAll l T3 T4)) venv0 (TAll l T1 T2) []) as A. {
+    clear H. clear H0.
+    unfold id in H5.
+    remember ((fresh venv1, (open (varF (fresh venv1)) T))::tenv0) as tenv.
+    assert (fresh tenv = S (fresh venv1)) as A. { rewrite Heqtenv. simpl. reflexivity. }
+    clear Heqtenv.
+    unfold id in H7.
+    remember ((fresh venv1, vobj venv1 (fresh venv1) ds) :: venv1) as venv.
+    assert (sstpd2 true venv (open (varF (fresh venv1)) T) venv0 (TAll l T1 T2) []) as B. { eexists; eassumption. }
+    clear H7. clear Heqvenv.
+    induction H5. destruct B as [? B]. inversion B.
+    simpl.
+    case_eq (le_lt_dec (fresh dcs) m); intros LE E1.
+    case_eq (beq_nat l m); intros E2.
+    exists y. eexists. eexists.
+    split. rewrite <- A. rewrite H0. reflexivity.
+    split. rewrite <- A. rewrite H0. eapply H.
+    destruct (tand_shape (TAll m T0 T3) TS).
+    rewrite H7 in H6. rewrite H6 in B. destruct B as [? B]. unfold open in B. simpl in B. inversion B. eapply beq_nat_true in E2. rewrite <- E2 in H11. eexists. eassumption.
+    eapply dcs_has_type_stp in H5. inversion H5. rewrite <- H4. eapply beq_nat_true in E2. rewrite <- E2. eexists. eassumption.
+    rewrite H7 in H6. rewrite H6 in B. eapply beq_nat_true in E2. rewrite <- E2 in B. apply B.
+    eapply IHdcs_has_type. apply A. destruct (tand_shape (TAll m T0 T3) TS).
+    rewrite H7 in H6. rewrite H6 in B. destruct B as [? B]. inversion B. unfold open in H11. simpl in H11. inversion H11. apply beq_nat_false in E2. omega. eexists. eassumption.
+    rewrite H7 in H6. rewrite H6 in B. destruct B as [? B]. inversion B. apply beq_nat_false in E2. omega.
+    inversion H5; subst. simpl in LE. omega. simpl in LE. omega. simpl in LE. omega.
+    simpl.
+    case_eq (le_lt_dec (fresh dcs) m); intros LE E1.
+    case_eq (beq_nat l m); intros E2.
+    destruct (tand_shape (TMem m T0 T0) TS).
+    rewrite H4 in H0. rewrite H0 in B. destruct B as [? B]. unfold open in B. simpl in B. inversion B. eapply beq_nat_true in E2. rewrite <- E2 in H9. inversion H9.
+    eapply dcs_has_type_stp in H5. inversion H5. rewrite <- H. eapply beq_nat_true in E2. rewrite <- E2. eexists. eassumption.
+    rewrite H4 in H0. rewrite H0 in B. eapply beq_nat_true in E2. rewrite <- E2 in B. inversion B.
+    unfold open in H6. simpl in H6. inversion H6.
+    eapply IHdcs_has_type. apply A. destruct (tand_shape (TMem m T0 T0) TS).
+    rewrite H4 in H0. rewrite H0 in B. destruct B as [? B]. inversion B. unfold open in H9. simpl in H9. inversion H9. eexists. eassumption.
+    rewrite H4 in H0. rewrite H0 in B. destruct B as [? B]. inversion B.
+    inversion H5; subst. simpl in LE. omega. simpl in LE. omega. simpl in LE. omega.
+  }
+  destruct A as [y [T3 [T4 [A1 [A2 A3]]]]].
+  exists (1 + (fresh venv1)). exists y. exists T3. exists T4.
+  split. reflexivity. split. reflexivity.
+  split. apply A1.
+  split. assumption. split. assumption.
+  split. eapply sstpd2_reg1. eexists. eassumption.
+  split. apply A2.
+  destruct A3 as [? A3]. inversion A3. subst. split.
+  eapply stpd2_upgrade. eexists. eassumption.
+
+  assert (stpd2 false venv0 T1
+          ((fresh venv1, vobj venv1 (fresh venv1) ds) :: venv1)
+          (open_rec 0 (varF (fresh venv1)) T3) []) as ARG. eauto.
+  assert (stpd2 false ((fresh venv1, vobj venv1 (fresh venv1) ds) :: venv1)
+          (open (varH 0) (open_rec 1 (varF (fresh venv1)) T4))
+          venv0 (open (varH 0) T2) [(0, (venv0, T1))]) as KEY. eauto.
+
+  eapply stpd2_upgrade in ARG.
+
+  assert (stpd2 false venv0 T1 venv0 T1 []) as HR1. eapply stpd2_wrapf. eapply stpd2_reg1. eauto.
+  assert (closed 0 0 T1). eapply stpd2_closed1 in HR1. simpl in HR1. apply HR1.
+
+  assert (stpd2 false ((1 + fresh venv1, vx)::(fresh venv1, vobj venv1 (fresh venv1) ds)::venv1)
+                (open_rec 0 (varF (1 + fresh venv1)) (open_rec 1 (varF (fresh venv1)) T4))
+                venv0 (open (varF xarg) T2) []) as HR2. {
+    eapply stpd2_substitute with (GH0:=nil).
+    eapply stpd2_extend1. eapply KEY.
+    eauto. simpl. eauto.
+    erewrite closed_no_subst. eassumption. eassumption.
+    eapply closed_upgrade_free. eauto. omega. eauto.
+    left. repeat eexists. eapply index_hit2. eauto. eauto. eauto.
+    rewrite closed_no_subst with (j:=0). eauto. eauto.
+    rewrite (subst_open_zero 0 1). eauto. eauto.
+    left. repeat eexists. eassumption.
+    rewrite closed_no_subst with (j:=0). eauto. eauto.
+    rewrite (subst_open_zero 0 1). eauto. eauto.
+    right. left. split. eauto. rewrite closed_no_subst with (j:=0). eauto. eauto.
+    eauto.
+  }
+  eapply stpd2_upgrade in HR2.
+  subst. eauto.
+Grab Existential Variables.
+apply 0. apply 0.
+Qed.
+
 Lemma valtp_reg: forall G v T n,
                    val_type G v T n ->
                    sstpd2 true G T G T [].
@@ -7487,6 +7595,36 @@ Proof.
       inversion HRY as [? vy].
 
       eapply not_stuck. eapply valtp_widen; eauto. rewrite EF. eauto.
+
+    +
+      remember (teval n venv0 e1) as tf.
+      remember (teval n venv0 (tvar x)) as tx.
+
+
+      destruct tx as [rx|]; try solve by inversion.
+      assert (res_type venv0 rx T1) as HRX. SCase "HRX". subst. eapply IHn; eauto.
+      inversion HRX as [? vx].
+
+      destruct tf as [rf|]; subst rx; try solve by inversion.
+      assert (res_type venv0 rf (TAll i T1 T2)) as HRF. SCase "HRF". subst. eapply IHn; eauto.
+      inversion HRF as [? vf].
+
+      destruct (invert_obj_var venv0 vf i T1 T2 n1 vx n0 x) as
+          [env1 [tenv [TF [ds [x0 [y0 [T3 [T4 [EF [FRX [EQDS [WF [HDS [HTF [HTY [STX STY]]]]]]]]]]]]]]]]. eauto. eauto.
+      admit.
+      eapply stpd2_upgrade. eapply stp_to_stp2. eassumption. eauto. eauto.
+      (* now we know it's a closure, and we have has_type evidence *)
+
+      assert (res_type ((x0,vx)::((fresh env1),vf)::env1) res (open (varF x0) (open_rec 1 (varF (fresh env1)) T4))) as HRY.
+        SCase "HRY".
+          subst. eapply IHn. rewrite EQDS in H3. eauto. eauto.
+          (* wf_env f x *) econstructor. eapply valtp_widen; eauto. eapply sstpd2_extend2. eauto. eauto.
+          (* wf_env f   *) econstructor. eapply v_obj; eauto.
+          eauto.
+      inversion HRY as [? vy].
+
+      eapply not_stuck. eapply valtp_widen; eauto. rewrite EF. eauto.
+
 
     + eapply restp_widen. eapply IHhas_type; eauto. eapply stpd2_upgrade. eapply stp_to_stp2; eauto.
 
